Clean up

Deque.thy
@@ -1,74 +1,6 @@
 theory Deque
-  imports Stack
+  imports State
 begin
-
-datatype 'a current = Current "'a list" nat "'a stack" nat
-
-datatype 'a state =
-  Norm "'a stack" nat |
-  RevB "'a current" "'a stack" "'a list" nat |
-  RevS1 "'a current" "'a stack" "'a list" |
-  RevS2 "'a current" "'a list" "'a stack" "'a list" nat |
-  Copy "'a current" "'a list" "'a list" nat
-
-fun put :: "'a \<Rightarrow> 'a current \<Rightarrow> 'a current" where
-  "put element (Current extra added old remained) = Current (element#extra) (added + 1) old remained"
-
-fun get :: "'a current \<Rightarrow> 'a * 'a current" where
-  "get (Current [] added old remained)     = (first old, Current [] added (pop old) (remained - 1))"
-| "get (Current (x#xs) added old remained) = (x, Current xs (added - 1) old remained)"
-
-fun top :: "'a current \<Rightarrow> 'a" where
-  "top current = (let (element, _) = get current in element)"
-
-fun bottom :: "'a current \<Rightarrow> 'a current" where
-  "bottom current = (let (_, bottom) = get current in bottom)"
-
-fun normalize :: "'a state \<Rightarrow> 'a state" where
-  "normalize (Copy current old new moved) = (
-      case current of Current extra added _ remained \<Rightarrow> 
-      if moved = remained
-      then Norm (Stack extra new) (added + moved)
-      else Copy current old new moved
-  )"
-| "normalize state = state"
-
-fun tick :: "'a state \<Rightarrow> 'a state" where
-  "tick state = (
-    case state of
-         Norm _ _ \<Rightarrow> state
-       | RevB current big auxB count \<Rightarrow> RevB current (pop big) ((first big)#auxB) (count - 1)
-       | RevS1 current small auxS \<Rightarrow> 
-          if isEmpty small 
-          then state 
-          else RevS1 current (pop small) ((first small)#auxS)
-       | RevS2 current auxS big newS count \<Rightarrow>
-          if isEmpty big
-          then normalize (Copy current auxS newS count)
-          else RevS2 current auxS (pop big) ((first big)#newS) (count + 1)
-       | Copy current aux new moved \<Rightarrow> case current of Current _ _ _ remained \<Rightarrow>
-          if moved < remained
-          then normalize (Copy current (tl aux) ((hd aux)#new) (moved + 1))
-          else normalize state
-  )"
-
-fun ticks :: "'a state \<Rightarrow> 'a state \<Rightarrow> 'a state * 'a state" where
-  "ticks (RevB currentB big auxB 0) (RevS1 currentS _ auxS) =
-    (normalize (Copy currentB auxB [] 0), RevS2 currentS auxS big [] 0)"
-| "ticks (RevS1 currentS _ auxS) (RevB currentB big auxB 0) =
-    (RevS2 currentS auxS big [] 0, normalize (Copy currentB auxB [] 0))"
-| "ticks left right = (tick left, tick right)"
-
-fun twice :: "('a \<Rightarrow> 'b \<Rightarrow> ('a * 'b)) \<Rightarrow> ('a \<Rightarrow> 'b \<Rightarrow> ('a * 'b))" where
-  "twice f = (\<lambda>a b. let (a', b') = f a b in f a' b')"
-
-definition fourTicks where
-  "fourTicks \<equiv> twice (twice ticks)"
-
-definition sixTicks where
-  "sixTicks \<equiv> twice (twice (twice ticks))"
-
-datatype side = Left | Right
 
 datatype 'a deque =
   Empty
@@ -89,36 +21,22 @@ fun swap :: "'a deque \<Rightarrow> 'a deque" where
 | "swap (One x) = One x"
 | "swap (Two x y) = Two y x"
 | "swap (Three x y z) = Three z y x"
-| "swap (Deque left right) = Deque left right"
+| "swap (Deque left right) = Deque right left"
 
-fun popState :: "'a state \<Rightarrow> 'a * 'a state" where
-  "popState (Norm a b)        = (first a, Norm (pop a) (b - 1))"
-| "popState (RevB a b c d)    = (top a,   RevB (bottom a) b c d)"
-| "popState (RevS1 a b c)     = (top a,   RevS1 (bottom a) b c)"
-| "popState (RevS2 a b c d e) = (top a,   RevS2 (bottom a) b c d e)"
-| "popState (Copy a b c d)    = (top a,   Copy (bottom a) b c d)"
+fun toSmallDeque :: "'a list \<Rightarrow> 'a list \<Rightarrow> 'a deque" where
+  "toSmallDeque []     [] = Empty"
 
-fun pushState :: "'a \<Rightarrow> 'a state \<Rightarrow> 'a state" where
-  "pushState x (Norm a b)        = Norm  (push x a) (Suc b)"
-| "pushState x (RevB a b c d)    = RevB  (put x a) b c d"
-| "pushState x (RevS1 a b c)     = RevS1 (put x a) b c"
-| "pushState x (RevS2 a b c d e) = RevS2 (put x a) b c d e"
-| "pushState x (Copy a b c d)    = Copy  (put x a) b c d"
+| "toSmallDeque (x#[]) [] = One x"
+| "toSmallDeque [] (x#[]) = One x"
 
-fun toSmall :: "'a list \<Rightarrow> 'a list \<Rightarrow> 'a deque" where
-  "toSmall []     [] = Empty"
+| "toSmallDeque (x#[])(y#[]) = Two y x"
+| "toSmallDeque (x#y#[]) [] = Two y x"
+| "toSmallDeque [] (x#y#[])= Two y x"
 
-| "toSmall (x#[]) [] = One x"
-| "toSmall [] (x#[]) = One x"
-
-| "toSmall (x#[])(y#[]) = Two y x"
-| "toSmall (x#y#[]) [] = Two y x"
-| "toSmall [] (x#y#[])= Two y x"
-
-| "toSmall [] (x#y#z#[])   = Three z y x"
-| "toSmall (x#y#z#[]) []   = Three z y x"
-| "toSmall (x#y#[]) (z#[]) = Three z y x"
-| "toSmall (x#[]) (y#z#[]) = Three z y x"
+| "toSmallDeque [] (x#y#z#[])   = Three z y x"
+| "toSmallDeque (x#y#z#[]) []   = Three z y x"
+| "toSmallDeque (x#y#[]) (z#[]) = Three z y x"
+| "toSmallDeque (x#[]) (y#z#[]) = Three z y x"
 
 fun dequeueLeft' :: "'a deque \<Rightarrow> 'a * 'a deque" where
   "dequeueLeft' (One x) = (x, Empty)"
@@ -130,10 +48,11 @@ fun dequeueLeft' :: "'a deque \<Rightarrow> 'a * 'a deque" where
     if 3 * (leftLength - 1) \<ge> rightLength 
     then (x, Deque (Norm left (leftLength - 1)) (Norm right rightLength))
     else if leftLength \<ge> 2
-    then let (left, newRight) = sixTicks (RevS1 (Current [] 0 left (2 * leftLength - 1)) left [])
-                                         (RevB  (Current [] 0 right (rightLength - leftLength)) right [] (rightLength - leftLength)) 
+    then let (left, newRight) =
+           sixTicks (RevS1 (Current [] 0 left (2 * leftLength - 1)) left [])
+                    (RevB  (Current [] 0 right (rightLength - leftLength)) right [] (rightLength - leftLength)) 
          in (x, Deque left newRight)
-    else case right of Stack r1 r2 \<Rightarrow> (x, toSmall r1 r2)
+    else case right of Stack r1 r2 \<Rightarrow> (x, toSmallDeque r1 r2)
   )"
 | "dequeueLeft' (Deque left right) = (
     let (x, left) = popState left in 
@@ -183,46 +102,35 @@ fun enqueueRight :: "'a \<Rightarrow> 'a deque \<Rightarrow> 'a deque" where
     in swap deque
   )"
 
-fun invar :: "'a deque \<Rightarrow> bool" where
-  "invar _ = True"
-
-lemma [simp]:"\<lbrakk>(x, deque') = dequeueLeft' (Deque left right)\<rbrakk>
-       \<Longrightarrow> size deque' < Suc (size left + size right)"
-  apply (
-        induction deque' arbitrary: x; 
-        induction left; 
-        induction right; 
-        auto simp: Let_def split: if_splits prod.splits stack.splits
-         )
-  sorry
-
-lemma [simp]:"\<lbrakk>(xa, y) = (case dequeueLeft' (Deque v va) of (x, deque) \<Rightarrow> (x, swap deque))\<rbrakk>
-       \<Longrightarrow> size y < Suc (size v + size va)"
-  sorry
-
-lemma [simp]: " \<lbrakk>(xa, y) = (case dequeueLeft' (List (rev vb @ [va])) of (x, deque) \<Rightarrow> (x, swap deque))\<rbrakk>
-       \<Longrightarrow> size y < Suc (Suc (length vb))"
-  sorry
+fun invariant :: "'a deque \<Rightarrow> bool" where
+  "invariant Empty = True"
+| "invariant (One _) = True"
+| "invariant (Two _ _) = True"
+| "invariant (Three _ _ _) = True"
+| "invariant (Deque (Norm left leftLength) (Norm right rightLength)) = (
+   size left = leftLength \<and>
+   size right = rightLength \<and>
+  (leftLength \<ge> 2 \<or> rightLength \<ge> 2) \<and>
+   (3 * rightLength \<ge> Suc leftLength \<or> 3 * leftLength \<ge> Suc rightLength)
+)"
+| "invariant _ = True"
 
 fun listLeft :: "'a deque \<Rightarrow> 'a list" where
   "listLeft Empty = []"
 | "listLeft (One x) = [x]"
 | "listLeft (Two x y) = [x, y]"
 | "listLeft (Three x y z) = [x, y, z]"
-| "listLeft deque = (
-    let (x, deque) = dequeueLeft' deque in
-      x # (listLeft deque)
-  )"
+| "listLeft (Deque left right) = (State.toList left) @ (rev (State.toList right))"
 
 fun listRight :: "'a deque \<Rightarrow> 'a list" where
   "listRight Empty = []"
 | "listRight (One x) = [x]"
 | "listRight (Two x y) = [y, x]"
 | "listRight (Three x y z) = [z, y, x]"
-| "listRight deque = (
-    let (x, deque) = dequeueRight' deque in
-      x # (listRight deque)
-  )"
+| "listRight (Deque left right) = (State.toList right) @ (rev (State.toList left))"
+
+(*
+For test purposes:
 
 fun enqueueLeftAll :: "'a list \<Rightarrow> 'a deque \<Rightarrow> 'a deque" where
   "enqueueLeftAll [] deque = deque"
@@ -235,103 +143,6 @@ fun enqueueRightAll :: "'a list \<Rightarrow> 'a deque \<Rightarrow> 'a deque" w
 fun dequeueLeftN :: "nat \<Rightarrow> 'a deque \<Rightarrow> 'a deque" where
   "dequeueLeftN 0 deque = deque"
 | "dequeueLeftN (Suc n) deque = dequeueLeftN n (dequeueLeft deque)" 
-
-locale Deque =
-fixes empty :: "'q"
-fixes enqueueLeft :: "'a \<Rightarrow> 'q \<Rightarrow> 'q"
-fixes enqueueRight :: "'a \<Rightarrow> 'q \<Rightarrow> 'q"
-fixes firstLeft :: "'q \<Rightarrow> 'a"
-fixes firstRight :: "'q \<Rightarrow> 'a"
-fixes dequeueLeft :: "'q \<Rightarrow> 'q"
-fixes dequeueRight :: "'q \<Rightarrow> 'q"
-fixes isEmpty :: "'q \<Rightarrow> bool"
-fixes listLeft :: "'q \<Rightarrow> 'a list"
-fixes listRight :: "'q \<Rightarrow> 'a list"
-(*fixes invar :: "'q \<Rightarrow> bool"*)
-assumes listLeft_empty:     "listLeft empty = []"
-assumes listRight_empty:    "listRight empty = []"
-assumes list_enqueueLeft:   "listLeft(enqueueLeft x q) = x # listLeft q"
-assumes list_enqueueRight:  "listRight(enqueueRight x q) = x # listRight q"
-assumes list_dequeueLeft:   "\<not> listLeft q = [] \<Longrightarrow> listLeft(dequeueLeft q) = tl(listLeft q)"
-assumes list_dequeueRight:  "\<not> listRight q = [] \<Longrightarrow> listRight(dequeueRight q) = tl(listRight q)"
-assumes list_firstLeft:     "\<not> listLeft q = [] \<Longrightarrow> firstLeft q = hd(listLeft q)"
-assumes list_firstRight:    "\<not> listRight q = [] \<Longrightarrow> firstRight q = hd(listRight q)"
-assumes listLeft_isEmpty:   "isEmpty q = (listLeft q = [])"
-assumes listRight_isEmpty:  "isEmpty q = (listRight q = [])"
-(*assumes invar_empty:        "invar empty"
-assumes invar_enqueueLeft:  "invar q \<Longrightarrow> invar(enqueueLeft x q)"
-assumes invar_enqueueRight: "invar q \<Longrightarrow> invar(enqueueRight x q)"
-assumes invar_dequeueLeft:  "invar q \<Longrightarrow> invar(dequeueLeft q)"
-assumes invar_dequeueRight: "invar q \<Longrightarrow> invar(dequeueRight q)"*)
-
-lemma "listLeft (dequeueLeft (enqueueLeft x deque)) = listLeft deque"
-  sorry
-
-interpretation RealtimeDeque: Deque where
-  empty    = empty    and
-  enqueueLeft = enqueueLeft and
-  enqueueRight = enqueueRight and
-  firstLeft = firstLeft and
-  firstRight = firstRight and
-  dequeueLeft = dequeueLeft and
-  dequeueRight = dequeueRight and
-  isEmpty = isEmpty and
-  listLeft = listLeft and
-  listRight = listRight
-proof (standard, goal_cases)
-case 1
-  then show ?case by(simp add: empty_def)
-next
-  case 2
-  then show ?case 
-    by(simp add: empty_def)
-next
-  case (3 x q)
-  then show ?case
-    apply(induction q arbitrary: x)
-    apply(auto split: prod.splits)
-    
-    sorry
-next
-  case (4 x q)
-  then show ?case
-    apply(induction q arbitrary: x)
-    apply (auto split: prod.splits)
-    sorry
-next
-  case (5 q)
-  then show ?case 
-    apply (auto split: prod.splits)
-    apply (induction q)
-    by auto
-next
-  case (6 q)
-  then show ?case 
-    apply (auto split: prod.splits)
-    apply (induction q)
-    by auto
-next
-  case (7 q)
-  then show ?case
-    apply (induction q)
-    by (auto split: prod.splits)
-next
-  case (8 q)
-  then show ?case 
-    apply(induction q)
-    by(auto split: prod.splits)
-next
-  case (9 q)
-  then show ?case
-    apply(induction q)
-    by(auto split: prod.splits)
-next
-  case (10 q)
-  then show ?case
-    apply(induction q)
-    by(auto split: prod.splits)
-qed
-
-
+*)
 
 end
