Stack.thy
@@ -22,4 +22,17 @@ fun first :: "'a stack \<Rightarrow> 'a" where
   "first (Stack (x#left) right)     = x"
 | "first (Stack []       (x#right)) = x"
 
+fun size :: "'a stack \<Rightarrow> nat" where
+  "size (Stack left right) = length left + length right"
+
+fun toList :: "'a stack \<Rightarrow> 'a list" where
+  "toList (Stack left right) = left @ right"
+
+fun invariant :: "'a stack \<Rightarrow> bool" where
+  "invariant (Stack [] []) = True"
+| "invariant (Stack [] _) = False"
+| "invariant _ = True"
+
+
+
 end
