Current.thy
@@ -1,0 +1,23 @@
+theory Current
+  imports Stack
+begin
+
+datatype 'a current = Current "'a list" nat "'a stack" nat
+
+fun put :: "'a \<Rightarrow> 'a current \<Rightarrow> 'a current" where
+  "put element (Current extra added old remained) = Current (element#extra) (added + 1) old remained"
+
+fun get :: "'a current \<Rightarrow> 'a * 'a current" where
+  "get (Current [] added old remained)     = (first old, Current [] added (pop old) (remained - 1))"
+| "get (Current (x#xs) added old remained) = (x, Current xs (added - 1) old remained)"
+
+fun top :: "'a current \<Rightarrow> 'a" where
+  "top current = (let (element, _) = get current in element)"
+
+fun bottom :: "'a current \<Rightarrow> 'a current" where
+  "bottom current = (let (_, bottom) = get current in bottom)"
+
+fun toList :: "'a current \<Rightarrow> 'a list" where
+  "toList (Current extra _ old _) = extra @ (Stack.toList old)"
+
+end
