Deque_Proof.thy
@@ -1,0 +1,288 @@
+theory Deque_Proof
+  imports Deque Stack_Proof
+begin
+
+locale Deque =
+fixes empty :: "'q"
+fixes enqueueLeft :: "'a \<Rightarrow> 'q \<Rightarrow> 'q"
+fixes enqueueRight :: "'a \<Rightarrow> 'q \<Rightarrow> 'q"
+fixes firstLeft :: "'q \<Rightarrow> 'a"
+fixes firstRight :: "'q \<Rightarrow> 'a"
+fixes dequeueLeft :: "'q \<Rightarrow> 'q"
+fixes dequeueRight :: "'q \<Rightarrow> 'q"
+fixes isEmpty :: "'q \<Rightarrow> bool"
+fixes listLeft :: "'q \<Rightarrow> 'a list"
+fixes listRight :: "'q \<Rightarrow> 'a list"
+fixes invariant :: "'q \<Rightarrow> bool"
+assumes listLeft_empty:     "listLeft empty = []"
+assumes listRight_empty:    "listRight empty = []"
+assumes list_enqueueLeft:   "invariant q \<Longrightarrow> listLeft(enqueueLeft x q) = x # listLeft q"
+assumes list_enqueueRight:  "invariant q \<Longrightarrow> listRight(enqueueRight x q) = x # listRight q"
+assumes list_dequeueLeft:   "invariant q \<Longrightarrow> \<not> listLeft q = [] \<Longrightarrow> listLeft(dequeueLeft q) = tl(listLeft q)"
+assumes list_dequeueRight:  "invariant q \<Longrightarrow> \<not> listRight q = [] \<Longrightarrow> listRight(dequeueRight q) = tl(listRight q)"
+assumes list_firstLeft:     "invariant q \<Longrightarrow> \<not> listLeft q = [] \<Longrightarrow> firstLeft q = hd(listLeft q)"
+assumes list_firstRight:    "invariant q \<Longrightarrow> \<not> listRight q = [] \<Longrightarrow> firstRight q = hd(listRight q)"
+assumes listLeft_isEmpty:   "invariant q \<Longrightarrow> isEmpty q = (listLeft q = [])"
+assumes listRight_isEmpty:  "invariant q \<Longrightarrow> isEmpty q = (listRight q = [])"
+assumes invariant_empty:        "invariant empty"
+assumes invariant_enqueueLeft:  "invariant q \<Longrightarrow> invariant(enqueueLeft x q)"
+assumes invariant_enqueueRight: "invariant q \<Longrightarrow> invariant(enqueueRight x q)"
+assumes invariant_dequeueLeft:  "invariant q \<Longrightarrow> \<not> isEmpty q  \<Longrightarrow> invariant(dequeueLeft q)"
+assumes invariant_dequeueRight: "invariant q \<Longrightarrow> \<not> isEmpty q  \<Longrightarrow> invariant(dequeueRight q)"
+
+lemma head: "xs \<noteq> [] \<Longrightarrow> hd xs = hd (xs @ ys)"
+  apply (induction xs arbitrary: ys)
+  by auto
+
+interpretation RealtimeDeque: Deque where
+  empty    = empty    and
+  enqueueLeft = enqueueLeft and
+  enqueueRight = enqueueRight and
+  firstLeft = firstLeft and
+  firstRight = firstRight and
+  dequeueLeft = dequeueLeft and
+  dequeueRight = dequeueRight and
+  isEmpty = isEmpty and
+  listLeft = listLeft and
+  listRight = listRight and
+  invariant = invariant
+proof (standard, goal_cases)
+case 1
+  then show ?case
+    by (simp add: empty_def)
+next
+case 2
+  then show ?case 
+    by (simp add: empty_def) 
+next
+  case (3 q x)
+  then show ?case 
+    proof (induction q arbitrary: x)
+      case Empty
+      then show ?case by simp 
+    next
+      case (One x)
+      then show ?case by simp
+    next
+      case (Two x y)
+      then show ?case by simp
+    next
+      case (Three x y z)
+      then show ?case by auto
+    next
+      case (Deque left right)
+      then show ?case
+      proof (induction left arbitrary: x)
+        case (Norm leftValues leftSize)
+        then show ?case
+        proof(induction right arbitrary: x)
+          case (Norm rightValues rightSize)
+          then show ?case 
+            apply (auto simp: push Let_def split: prod.splits)
+            sorry
+        next
+          case (RevB x1 x2 x3 x4)
+          then show ?case sorry
+        next
+          case (RevS1 x1 x2 x3)
+          then show ?case sorry
+        next
+          case (RevS2 x1 x2 x3 x4 x5)
+          then show ?case sorry
+        next
+          case (Copy x1 x2 x3 x4)
+          then show ?case sorry
+        qed
+      next
+        case (RevB x1 x2 x3 x4)
+        then show ?case sorry
+      next
+        case (RevS1 x1 x2 x3)
+        then show ?case sorry
+      next
+        case (RevS2 x1 x2 x3 x4 x5)
+        then show ?case sorry
+      next
+        case (Copy x1 x2 x3 x4)
+        then show ?case sorry
+      qed
+    qed
+next
+  case (4 q x)
+  then show ?case
+  proof (induction q arbitrary: x)
+      case Empty
+      then show ?case by auto
+    next
+      case (One x)
+      then show ?case by auto
+    next
+      case (Two x y)
+      then show ?case by auto
+    next
+      case (Three x y z)
+      then show ?case by auto
+    next
+      case (Deque left right)
+      then show ?case sorry
+    qed
+next
+  case (5 q)
+  then show ?case 
+  proof(induction q)
+    case Empty
+    then show ?case by auto
+  next
+    case (One x)
+    then show ?case by auto
+  next
+    case (Two x1 x2a)
+    then show ?case by auto
+  next
+    case (Three x1 x2a x3)
+    then show ?case by auto
+  next
+    case (Deque left right)
+    then show ?case 
+    proof(induction left)
+      case (Norm leftValues leftLength)
+      then show ?case 
+      proof(induction right arbitrary: leftValues leftValues)
+        case (Norm rightValues rightLength)
+        then show ?case
+          (*apply(auto simp: Let_def pop not_empty split: prod.splits stack.splits)*)
+          sorry
+        next
+          case (RevB x1 x2 x3 x4)
+          then show ?case sorry
+        next
+          case (RevS1 x1 x2 x3)
+          then show ?case sorry
+        next
+          case (RevS2 x1 x2 x3 x4 x5)
+          then show ?case sorry
+        next
+          case (Copy x1 x2 x3 x4)
+          then show ?case sorry
+        qed        
+    next
+      case (RevB x1 x2 x3 x4)
+      then show ?case sorry
+    next
+      case (RevS1 x1 x2 x3)
+      then show ?case sorry
+    next
+      case (RevS2 x1 x2 x3 x4 x5)
+      then show ?case sorry
+    next
+      case (Copy x1 x2 x3 x4)
+      then show ?case sorry
+    qed  
+  qed
+next
+  case (6 q)
+  then show ?case sorry
+next
+  case (7 q)
+  then show ?case
+  proof(induction q)
+    case Empty
+    then show ?case by auto
+  next
+    case (One x)
+    then show ?case by auto
+  next
+    case (Two x1 x2a)
+    then show ?case by auto
+  next
+    case (Three x1 x2a x3)
+    then show ?case by auto
+  next
+    case (Deque left right)
+    then show ?case 
+      apply(induction left; induction right)
+      (*apply(auto simp: Let_def first head not_empty not_empty_2 empty split: prod.splits stack.splits)*)
+      sorry
+  qed
+next
+  case (8 q)
+  then show ?case sorry
+next
+  case (9 q)
+  then show ?case 
+  proof induction
+    case Empty
+    then show ?case by auto
+  next
+    case (One x)
+    then show ?case by auto
+  next
+    case (Two x1 x2a)
+    then show ?case by auto
+  next
+    case (Three x1 x2a x3)
+    then show ?case by auto
+  next
+    case (Deque left right)
+    then show ?case 
+  
+      apply auto sorry
+  qed 
+next
+  case (10 q)
+  then show ?case sorry
+next
+  case 11
+  then show ?case 
+    by (simp add: empty_def)
+next
+  case (12 q x)
+  then show ?case
+  proof(induction q arbitrary: x)
+  case Empty
+  then show ?case by auto
+  next
+    case (One x)
+    then show ?case by auto
+  next
+    case (Two x1 x2a)
+    then show ?case by auto
+  next
+    case (Three x1 x2a x3)
+    then show ?case by auto
+  next
+  case (Deque left right)
+  then show ?case
+    sorry
+  qed
+next
+  case (13 q x)
+  then show ?case sorry
+next
+  case (14 q)
+  then show ?case
+  proof(induction q)
+    case Empty
+    then show ?case by auto
+  next
+    case (One x)
+    then show ?case by auto
+  next
+    case (Two x1 x2a)
+  then show ?case by auto
+  next
+  case (Three x1 x2a x3)
+  then show ?case by auto
+  next
+  case (Deque left right)
+  then show ?case 
+    apply(induction left; induction right)
+    apply (auto simp: Let_def split: stack.splits prod.splits)
+    sorry
+  qed
+next
+  case (15 q)
+  then show ?case sorry
+qed
+
+end
