Stack_Proof.thy
@@ -1,0 +1,49 @@
+theory Stack_Proof
+  imports Stack
+begin
+
+lemma push: "toList (push x stack) = x # toList stack"
+  apply(induction stack arbitrary: x)
+  by auto
+
+lemma pop: "\<not> isEmpty stack \<Longrightarrow> toList (pop stack) = tl (toList stack)"
+proof(induction stack)
+  case (Stack left right)
+  then show ?case 
+    apply(induction left; induction right)
+    by auto
+qed
+
+lemma not_empty: "size stack > 0 \<Longrightarrow> \<not> isEmpty stack"
+proof(induction stack)
+  case (Stack left right)
+  then show ?case
+    apply(induction left; induction right)
+    by auto
+qed
+
+lemma not_empty_2: "\<not> Stack.isEmpty stack \<Longrightarrow> Stack.toList stack  \<noteq> []"
+  apply (induction stack)
+  by auto
+
+lemma size_push: "size (push x stack) = Suc (size stack)"
+  apply(induction stack arbitrary: x)
+  by auto
+
+lemma first: "\<not> isEmpty stack \<Longrightarrow> first stack = hd (toList stack)"
+proof(induction stack)
+  case (Stack left right)
+  then show ?case
+    apply(induction left; induction right)
+    by auto
+qed
+
+lemma empty: "toList stack \<noteq> [] \<Longrightarrow> \<not>isEmpty stack"
+proof(induction stack)
+  case (Stack left right)
+  then show ?case
+    apply(induction left; induction right)
+    by auto
+qed
+
+end
